thys/JinjaThreads/Execute/TypeRelRefine.thy
@@ -1,7 +1,7 @@
 theory TypeRelRefine imports
   "../Common/TypeRel"
   "~~/src/HOL/Library/AssocList"
-  "~~/src/HOL/Library/Cset"
+  "~~/src/HOL/Library/List_Cset"
 begin
 
 subsection {* Auxiliary lemmata *}
